src/Examples/Layouts/GridLayout.v
@@ -1,6 +1,6 @@
 From Stdlib Require Import List Bool Lia.
 From Datalog Require Import Datalog.
-From DatalogRocq Require Import Dataflow Graph GridGraph.
+From DatalogRocq Require Import DistributedDatalog Graph GridGraph ConnectedTopology.
 From coqutil Require Import Map.Interface.
 Import ListNotations.
 
@@ -41,7 +41,7 @@ Section GridLayout.
   Definition mk_always_forward_table (dims : list nat) (n : Node) : rel -> list Node :=
     fun f => filter (GridGraph.is_neighbor dims n) (all_nodes_h dims).
 
-  Definition mk_no_input_fn (n : Node) (f : rel * (list T)) : Prop := False.
+  Definition mk_no_input_fn (n : Node) (f : Datalog.fact rel T) : Prop := False.
 
   Definition mk_all_output_fn (n : Node) (f : rel) : Prop := True.
 
@@ -49,13 +49,13 @@ Section GridLayout.
   Definition mk_dataflow_network
              (dims : list nat)
              (indexed_layout : list (Node * list nat))
-             (program : list rule) : Dataflow.DataflowNetwork :=
+             (program : list rule) : DistributedDatalog.DataflowNetwork :=
     {|
-      Dataflow.graph := mk_grid_graph dims;
-      Dataflow.layout := mk_layout_from_indexed_layout dims indexed_layout program;
-      Dataflow.forward := mk_always_forward_table dims;
-      Dataflow.input := mk_no_input_fn;
-      Dataflow.output := mk_all_output_fn
+      DistributedDatalog.graph := mk_grid_graph dims;
+      DistributedDatalog.layout := mk_layout_from_indexed_layout dims indexed_layout program;
+      DistributedDatalog.forward := mk_always_forward_table dims;
+      DistributedDatalog.input := mk_no_input_fn;
+      DistributedDatalog.output := mk_all_output_fn
     |}.
 
   Definition rule_in_layout (r : rule) (layout : Node -> list rule) (dims : list nat): bool :=
@@ -85,10 +85,10 @@ Section GridLayout.
 Theorem good_layout :
     forall dims indexed_layout program,
     check_layout dims (mk_layout_from_indexed_layout dims indexed_layout program) program = true ->
-    Dataflow.good_layout (mk_layout_from_indexed_layout dims indexed_layout program) (GridGraph dims).(nodes) program.
+    DistributedDatalog.good_layout (mk_layout_from_indexed_layout dims indexed_layout program) (GridGraph dims).(nodes) program.
 Proof.
     unfold check_layout.
-    unfold Dataflow.good_layout.
+    unfold DistributedDatalog.good_layout.
     intros.
     split.
     - apply Forall_forall. intros. apply andb_true_iff in H. destruct H as [H_nodes_ok H_rule_in_layout].
@@ -188,7 +188,7 @@ Proof.
   split.
   - intros n_prod n_cons Hprod Hcons.
   assert (Hn_prod : GridGraph.is_graph_node dims0 n_prod).
-  { destruct Hprod as [r [concl [Hin_layout [_ _]]]].
+  { destruct Hprod as [r [Hin_layout _]].
     eapply layout_nonempty_only_valid_nodes; apply Hin_layout. }
   assert (Hn_cons : GridGraph.is_graph_node dims0 n_cons).
   { destruct Hcons as [r [Hin_layout _]].
@@ -203,7 +203,7 @@ Qed.
 Lemma good_network :
   forall dims indexed_layout program,
   check_layout dims (mk_layout_from_indexed_layout dims indexed_layout program) program = true ->
-  Dataflow.good_network (mk_dataflow_network dims indexed_layout program) program.
+  DistributedDatalog.good_network (mk_dataflow_network dims indexed_layout program) program.
 Proof.
   intros dims indexed_layout program Hcheck.
   unfold mk_dataflow_network. unfold good_network.
@@ -223,34 +223,95 @@ Proof.
       * split.
         ** simpl. unfold good_input. intros. inversion H.
         ** simpl. unfold good_output. intros. exists n. split.
-            --- destruct H as [r [concl [Hin_layout _]]].
+            --- destruct H as [r [Hin_layout _]].
              apply layout_nonempty_only_valid_nodes in Hin_layout.
              exact Hin_layout.
            --- simpl. unfold mk_all_output_fn. trivial.
 Qed.
 
-Theorem soundness :
-    forall dims indexed_layout program,
-    check_layout dims (mk_layout_from_indexed_layout dims indexed_layout program) program = true ->
-    forall f,
-    network_prog_impl_fact (mk_dataflow_network dims indexed_layout program) f ->
-    prog_impl_fact program f.
+(*===========================================================================*)
+(*  THE GRID AS A [connected_topology] INSTANCE                              *)
+(*                                                                           *)
+(*  We discharge each field of the abstract interface for the grid, then     *)
+(*  package them as [grid_topology].  From that point on, [good_network] for  *)
+(*  the grid is just [good_network_ct grid_topology] -- no grid reasoning is  *)
+(*  redone, and the very same generic theorem serves any other topology.     *)
+(*===========================================================================*)
+
+Lemma grid_all_nodes_spec (dims : Dimensions) :
+  forall n, In n (all_nodes_h dims) <-> (GridGraph dims).(nodes) n.
+Proof. intros n. symmetry. apply GridGraph.all_nodes_h_correct. Qed.
+
+Lemma grid_forward_sound (dims : Dimensions) :
+  forall n1 n2 r, In n2 (mk_always_forward_table dims n1 r) ->
+    (GridGraph dims).(nodes) n1 /\ (GridGraph dims).(nodes) n2 /\ (GridGraph dims).(edge) n1 n2.
 Proof.
-  intros dims indexed_layout program Hcheck f Hnetwork.
-  apply (Dataflow.soundness (mk_dataflow_network dims indexed_layout program) program); auto.
-  apply good_network; auto.
+  intros n1 n2 r H. unfold mk_always_forward_table in H.
+  apply filter_In in H. destruct H as [Hneighbor Hin].
+  apply GridGraph.is_neighbor_correct in Hin.
+  split; try inversion Hin; auto.
 Qed.
 
-Theorem completeness :
-    forall dims indexed_layout program,
-    check_layout dims (mk_layout_from_indexed_layout dims indexed_layout program) program = true ->
-    forall f,
-    prog_impl_fact program f ->
-    network_prog_impl_fact (mk_dataflow_network dims indexed_layout program) f.
+Lemma grid_connected_topology (dims : Dimensions) :
+  forall r n1 n2, (GridGraph dims).(nodes) n1 -> (GridGraph dims).(nodes) n2 ->
+    n1 = n2 \/ forwarding_reachable (mk_always_forward_table dims) r n1 n2.
 Proof.
-  intros dims indexed_layout program Hcheck f Hprog.
-  apply (Dataflow.completeness (mk_dataflow_network dims indexed_layout program) program); auto.
-  apply good_network; auto.
+  intros r n1 n2 H1 H2.
+  apply grid_reachable_to_forwarding.
+  apply GridGraph.grid_connected; auto.
 Qed.
+
+Lemma grid_no_input (dims : Dimensions) :
+  forall n f, ~ mk_no_input_fn n f.
+Proof. intros n f H. exact H. Qed.
+
+Lemma grid_output_total (dims : Dimensions) :
+  forall n r, (GridGraph dims).(nodes) n -> mk_all_output_fn n r.
+Proof. intros n r _. exact I. Qed.
+
+(* The grid, packaged as an abstract connected topology.  [input_node] is the (real) node where
+   streaming base facts enter -- any real node works, by connectivity. *)
+Definition grid_topology (dims : Dimensions) (input_node : Node)
+    (Hinput : (GridGraph dims).(nodes) input_node) : connected_topology :=
+  {| ct_graph         := GridGraph dims;
+     ct_forward       := mk_always_forward_table dims;
+     ct_input         := mk_no_input_fn;
+     ct_output        := mk_all_output_fn;
+     ct_all_nodes     := all_nodes_h dims;
+     ct_all_nodes_spec := grid_all_nodes_spec dims;
+     ct_good_graph    := GridGraph.good_graph dims;
+     ct_forward_sound := grid_forward_sound dims;
+     ct_connected     := grid_connected_topology dims;
+     ct_no_input      := grid_no_input dims;
+     ct_output_total  := grid_output_total dims;
+     ct_input_node      := fun _ => input_node;
+     ct_input_node_real := fun _ => Hinput |}.
+
+(* [good_network] for the grid is now a one-liner through the generic theorem. *)
+Theorem grid_good_network (dims : Dimensions) (input_node : Node)
+    (Hinput : (GridGraph dims).(nodes) input_node)
+    (L : Node -> list rule) (program : list rule) :
+  ConnectedTopology.layout_valid_nodes (grid_topology dims input_node Hinput) L ->
+  ConnectedTopology.check_layout (rule_eqb := rule_eqb) (grid_topology dims input_node Hinput) L program = true ->
+  DistributedDatalog.good_network (net_of (grid_topology dims input_node Hinput) L) program.
+Proof.
+  intros Hvalid Hcheck. apply (good_network_ct (rule_eqb := rule_eqb)); assumption.
+Qed.
+
+(* [good_network_streaming] for the grid, for any base facts [Q] entering at [input_node]. *)
+Theorem grid_good_network_streaming (dims : Dimensions) (input_node : Node)
+    (Hinput : (GridGraph dims).(nodes) input_node)
+    (L : Node -> list rule) (program : list rule) (Q : Datalog.fact rel T -> Prop) :
+  ConnectedTopology.layout_valid_nodes (grid_topology dims input_node Hinput) L ->
+  ConnectedTopology.check_layout (rule_eqb := rule_eqb) (grid_topology dims input_node Hinput) L program = true ->
+  DistributedDatalog.good_network_streaming
+    (net_of_streaming (grid_topology dims input_node Hinput) L Q) program Q.
+Proof.
+  intros Hvalid Hcheck. apply (good_network_streaming_ct (rule_eqb := rule_eqb)); assumption.
+Qed.
+
+(* (The grid's bespoke soundness/completeness convenience theorems were removed: they duplicated
+   the generic [ConnectedTopology] streaming theorems -- use [grid_good_network_streaming] with
+   [ConnectedTopology]/[EncodeLayoutCorrect.compile_checked_correct] instead.) *)
 
 End GridLayout.
